venom/passes/simplify_cfg/scfgCorrectScript.sml
@@ -1,439 +1,378 @@
-(*
+(* 
  * Simplify-CFG Correctness
  *
- * This theory proves basic correctness lemmas for simplify-cfg steps.
+ * Pass-level correctness theorems for simplify-cfg.
  *)
 
 Theory scfgCorrect
 Ancestors
-  scfgDefs scfgTransform list relation stateEquiv venomSem venomState venomInst finite_map
+  scfgMergeCorrect scfgTransform list relation
 
-(* ===== Equivalence Basics ===== *)
+(* ===== CFG/Lookup Helpers ===== *)
 
-Theorem state_equiv_cfg_refl:
-  !s. state_equiv_cfg s s
+Theorem lookup_block_label:
+  !lbl blocks bb.
+    lookup_block lbl blocks = SOME bb ==> bb.bb_label = lbl
 Proof
-  rw[state_equiv_cfg_def, var_equiv_def]
-QED
-
-Theorem state_equiv_cfg_sym:
-  !s1 s2. state_equiv_cfg s1 s2 ==> state_equiv_cfg s2 s1
-Proof
-  rw[state_equiv_cfg_def, var_equiv_def]
-QED
-
-Theorem state_equiv_cfg_trans:
-  !s1 s2 s3.
-    state_equiv_cfg s1 s2 /\ state_equiv_cfg s2 s3 ==> state_equiv_cfg s1 s3
-Proof
-  rw[state_equiv_cfg_def, var_equiv_def] >> metis_tac[]
-QED
-
-Theorem result_equiv_cfg_refl:
-  !r. result_equiv_cfg r r
-Proof
-  Cases >> rw[result_equiv_cfg_def, state_equiv_cfg_refl]
-QED
-
-Theorem result_equiv_cfg_trans:
-  !r1 r2 r3. result_equiv_cfg r1 r2 /\ result_equiv_cfg r2 r3 ==> result_equiv_cfg r1 r3
-Proof
-  Cases >> Cases >> Cases >>
-  simp[result_equiv_cfg_def] >> metis_tac[state_equiv_cfg_trans]
-QED
-
-(* ===== Operand Evaluation under state_equiv_cfg ===== *)
-
-Theorem eval_operand_state_equiv_cfg:
-  !op s1 s2.
-    state_equiv_cfg s1 s2 ==> eval_operand op s1 = eval_operand op s2
-Proof
-  Cases_on `op` >>
-  rw[eval_operand_def, state_equiv_cfg_def, var_equiv_def]
-QED
-
-(* ===== State Operations Preserve state_equiv_cfg ===== *)
-
-Theorem update_var_state_equiv_cfg:
-  !x v s1 s2.
-    state_equiv_cfg s1 s2 ==>
-    state_equiv_cfg (update_var x v s1) (update_var x v s2)
-Proof
-  rw[state_equiv_cfg_def, var_equiv_def, update_var_def, lookup_var_def, FLOOKUP_UPDATE]
-QED
-
-Theorem mstore_state_equiv_cfg:
-  !offset v s1 s2.
-    state_equiv_cfg s1 s2 ==>
-    state_equiv_cfg (mstore offset v s1) (mstore offset v s2)
-Proof
-  rw[state_equiv_cfg_def, var_equiv_def, mstore_def, lookup_var_def]
-QED
-
-Theorem sstore_state_equiv_cfg:
-  !key v s1 s2.
-    state_equiv_cfg s1 s2 ==>
-    state_equiv_cfg (sstore key v s1) (sstore key v s2)
-Proof
-  rw[state_equiv_cfg_def, var_equiv_def, sstore_def, lookup_var_def]
-QED
-
-Theorem tstore_state_equiv_cfg:
-  !key v s1 s2.
-    state_equiv_cfg s1 s2 ==>
-    state_equiv_cfg (tstore key v s1) (tstore key v s2)
-Proof
-  rw[state_equiv_cfg_def, var_equiv_def, tstore_def, lookup_var_def]
-QED
-
-Theorem write_memory_with_expansion_state_equiv_cfg:
-  !offset bytes s1 s2.
-    state_equiv_cfg s1 s2 ==>
-    state_equiv_cfg (write_memory_with_expansion offset bytes s1)
-                    (write_memory_with_expansion offset bytes s2)
-Proof
-  rw[state_equiv_cfg_def, var_equiv_def, write_memory_with_expansion_def, lookup_var_def]
-QED
-
-Theorem jump_to_state_equiv_cfg:
-  !lbl1 lbl2 s1 s2.
-    state_equiv_cfg s1 s2 ==>
-    state_equiv_cfg (jump_to lbl1 s1) (jump_to lbl2 s2)
-Proof
-  rw[state_equiv_cfg_def, var_equiv_def, jump_to_def, lookup_var_def]
-QED
-
-Theorem halt_state_state_equiv_cfg:
-  !s1 s2.
-    state_equiv_cfg s1 s2 ==>
-    state_equiv_cfg (halt_state s1) (halt_state s2)
-Proof
-  rw[state_equiv_cfg_def, var_equiv_def, halt_state_def, lookup_var_def]
-QED
-
-Theorem revert_state_state_equiv_cfg:
-  !s1 s2.
-    state_equiv_cfg s1 s2 ==>
-    state_equiv_cfg (revert_state s1) (revert_state s2)
-Proof
-  rw[state_equiv_cfg_def, var_equiv_def, revert_state_def, lookup_var_def]
-QED
-
-(* ===== resolve_phi under Label Rewriting ===== *)
-
-Theorem resolve_phi_replace_label:
-  !old new ops v.
-    old <> new /\
-    ~MEM (Label new) ops /\
-    resolve_phi old ops = SOME (Var v) ==>
-    resolve_phi new (MAP (replace_label_operand old new) ops) =
-    SOME (Var v)
-Proof
-  measureInduct_on `LENGTH ops` >>
-  Cases_on `ops` >- simp[resolve_phi_def] >>
-  Cases_on `t` >- simp[resolve_phi_def] >>
-  rename1 `h::h2::t2` >>
-  Cases_on `h` >> Cases_on `h2` >>
+  Induct_on `blocks` >> simp[lookup_block_def] >>
   rpt strip_tac >>
-  fs[resolve_phi_def, replace_label_operand_def] >>
-  TRY (Cases_on `s = old` >> fs[]) >>
-  TRY (Cases_on `s = new` >> fs[]) >>
-  simp[resolve_phi_def] >>
-  `LENGTH t2 < LENGTH (h::h2::t2)` by simp[] >>
-  `~MEM (Label new) t2` by simp[] >>
+  Cases_on `h.bb_label = lbl` >> fs[]
+QED
+
+Theorem lookup_block_MEM:
+  !lbl blocks bb.
+    lookup_block lbl blocks = SOME bb ==> MEM bb blocks
+Proof
+  Induct_on `blocks` >> simp[lookup_block_def] >>
+  rpt strip_tac >> Cases_on `h.bb_label = lbl` >> fs[] >>
   res_tac >> simp[]
 QED
 
-(* TODO: proof attempt
+Theorem lookup_block_at_hd:
+  !lbl blocks bb.
+    blocks <> [] /\
+    lbl = (HD blocks).bb_label /\
+    lookup_block lbl blocks = SOME bb ==>
+    bb = HD blocks
 Proof
-  measureInduct_on `LENGTH ops` >>
-  Cases_on `ops` >- simp[resolve_phi_def] >>
-  Cases_on `t` >- simp[resolve_phi_def] >>
-  Cases_on `h` >> Cases_on `h'` >>
+  Cases_on `blocks` >> simp[lookup_block_def]
+QED
+
+Theorem lookup_block_filter:
+  !P lbl blocks bb.
+    lookup_block lbl blocks = SOME bb /\ P bb ==>
+    lookup_block lbl (FILTER P blocks) = SOME bb
+Proof
+  Induct_on `blocks` >> simp[lookup_block_def] >>
   rpt strip_tac >>
-  fs[resolve_phi_def, replace_label_operand_def] >>
-  TRY (
-    Cases_on `s = old` >> fs[] >>
-    first_x_assum (qspec_then `t'` mp_tac) >> simp[] >>
-    strip_tac >> simp[]
-  ) >>
-  first_x_assum (qspec_then `t'` mp_tac) >> simp[] >>
-  strip_tac >> simp[]
-QED
-*)
-
-Theorem resolve_phi_remove_non_preds:
-  !preds prev ops val.
-    MEM prev preds /\
-    resolve_phi prev ops = SOME val ==>
-    resolve_phi prev (phi_remove_non_preds preds ops) = SOME val
-Proof
-  measureInduct_on `LENGTH ops` >>
-  Cases_on `ops` >- simp[resolve_phi_def, phi_remove_non_preds_def] >>
-  Cases_on `t` >- simp[resolve_phi_def, phi_remove_non_preds_def] >>
-  rename1 `h::h2::t2` >>
-  Cases_on `h`
-  >- fs[resolve_phi_def, phi_remove_non_preds_def]
-  >- fs[resolve_phi_def, phi_remove_non_preds_def]
-  >- (
-    rpt strip_tac >>
-    Cases_on `s = prev`
-    >- fs[resolve_phi_def, phi_remove_non_preds_def]
-    >- (
-      qpat_x_assum `resolve_phi prev (Label s::h2::t2) = SOME val` mp_tac >>
-      simp[resolve_phi_def] >>
-      strip_tac >>
-      qpat_x_assum
-        `!ops'. LENGTH ops' < LENGTH (Label s::h2::t2) ==> _` mp_tac >>
-      disch_then (qspec_then `t2` mp_tac) >>
-      simp[] >>
-      disch_then (qspecl_then [`preds`, `prev`, `val`] mp_tac) >>
-      strip_tac >>
-      Cases_on `MEM s preds`
-      >- simp[resolve_phi_def, phi_remove_non_preds_def]
-      >- fs[resolve_phi_def, phi_remove_non_preds_def]
-    )
-  )
+  Cases_on `h.bb_label = lbl` >> fs[]
+  >- (fs[] >> simp[lookup_block_def])
+  >- (first_x_assum drule >> simp[])
 QED
 
-(* TODO: proof attempt
+Theorem lookup_block_filter_none:
+  !P lbl blocks.
+    lookup_block lbl blocks = NONE ==> lookup_block lbl (FILTER P blocks) = NONE
 Proof
-  measureInduct_on `LENGTH ops` >>
-  Cases_on `ops` >- simp[resolve_phi_def, phi_remove_non_preds_def] >>
-  Cases_on `t` >- simp[resolve_phi_def, phi_remove_non_preds_def] >>
-  Cases_on `h` >> Cases_on `h'` >>
+  Induct_on `blocks` >> simp[lookup_block_def] >>
   rpt strip_tac >>
-  fs[resolve_phi_def, phi_remove_non_preds_def] >>
-  TRY (
-    Cases_on `s = prev` >> fs[] >>
-    first_x_assum (qspec_then `t'` mp_tac) >> simp[] >>
-    strip_tac >> simp[]
-  ) >>
-  first_x_assum (qspec_then `t'` mp_tac) >> simp[] >>
-  strip_tac >> simp[]
+  Cases_on `h.bb_label = lbl` >> fs[]
 QED
-*)
 
-(* ===== PHI Simplification Preserves Step ===== *)
-
-Theorem step_inst_simplify_phi_inst:
-  !preds inst s prev out val_op.
-    inst.inst_opcode = PHI /\
-    inst.inst_outputs = [out] /\
-    s.vs_prev_bb = SOME prev /\
-    MEM prev preds /\
-    resolve_phi prev inst.inst_operands = SOME val_op
-  ==>
-    result_equiv_cfg (step_inst (simplify_phi_inst preds inst) s)
-                     (step_inst inst s)
+Theorem lookup_block_simplify_phi_block:
+  !lbl blocks fn' bb.
+    lookup_block lbl blocks = SOME bb ==>
+    lookup_block lbl
+      (MAP (\\bb. simplify_phi_block (pred_labels fn' bb.bb_label) bb) blocks) =
+    SOME (simplify_phi_block (pred_labels fn' lbl) bb)
 Proof
+  Induct_on `blocks` >> simp[lookup_block_def] >>
   rpt strip_tac >>
-  simp[simplify_phi_inst_def] >>
-  qabbrev_tac `ops = phi_remove_non_preds preds inst.inst_operands` >>
-  sg `resolve_phi prev ops = SOME val_op`
-  >- (
-    fs[Abbr`ops`] >>
-    irule resolve_phi_remove_non_preds >> simp[]
-  )
-  >- (
-    Cases_on `ops`
-    >- fs[resolve_phi_def]
-    >- (
-      Cases_on `t`
-      >- fs[resolve_phi_def]
-      >- (
-        rename1 `h::h2::t2` >>
-        Cases_on `t2`
-        >- (
-          Cases_on `h`
-          >- fs[resolve_phi_def]
-          >- fs[resolve_phi_def]
-          >- (
-            fs[step_inst_def, resolve_phi_def, result_equiv_cfg_def] >>
-            simp[result_equiv_cfg_def, state_equiv_cfg_def, var_equiv_def] >>
-            Cases_on `eval_operand val_op s`
-            >- simp[result_equiv_cfg_def, state_equiv_cfg_def, var_equiv_def]
-            >- simp[result_equiv_cfg_def, state_equiv_cfg_def, var_equiv_def]
-          )
-        )
-        >- (
-          fs[step_inst_def, result_equiv_cfg_def, state_equiv_cfg_def,
-             var_equiv_def] >>
-          Cases_on `eval_operand val_op s`
-          >- simp[result_equiv_cfg_def, state_equiv_cfg_def, var_equiv_def]
-          >- simp[result_equiv_cfg_def, state_equiv_cfg_def, var_equiv_def]
-        )
-      )
-    )
-  )
+  Cases_on `h.bb_label = lbl` >> fs[lookup_block_label]
+  >- simp[lookup_block_def, simplify_phi_block_label]
+  >- (first_x_assum drule >> simp[])
 QED
 
-(* TODO: proof attempt
+Theorem lookup_block_simplify_phi_block_none:
+  !lbl blocks fn'.
+    lookup_block lbl blocks = NONE ==>
+    lookup_block lbl
+      (MAP (\\bb. simplify_phi_block (pred_labels fn' bb.bb_label) bb) blocks) = NONE
+Proof
+  Induct_on `blocks` >> simp[lookup_block_def] >>
+  rpt strip_tac >>
+  Cases_on `h.bb_label = lbl` >> fs[lookup_block_def, simplify_phi_block_label]
+QED
+
+Theorem pred_labels_mem_from_edge:
+  !fn bb lbl.
+    MEM bb fn.fn_blocks /\ MEM lbl (block_successors bb) ==>
+    MEM bb.bb_label (pred_labels fn lbl)
+Proof
+  rw[pred_labels_def] >>
+  simp[MEM_MAP] >>
+  qexists_tac `bb` >>
+  simp[MEM_FILTER]
+QED
+
+Theorem pred_labels_subset:
+  !fn fn' lbl pred.
+    (!bb. MEM bb fn'.fn_blocks ==> MEM bb fn.fn_blocks) /\
+    MEM pred (pred_labels fn' lbl) ==>
+    MEM pred (pred_labels fn lbl)
+Proof
+  rw[pred_labels_def] >>
+  fs[MEM_MAP, MEM_FILTER] >>
+  metis_tac[]
+QED
+
+Theorem pred_labels_keep_reachable:
+  !fn entry lbl prev keep.
+    keep = FILTER (\\bb. reachable_label fn entry bb.bb_label) fn.fn_blocks /\
+    MEM prev (pred_labels fn lbl) /\
+    reachable_label fn entry prev ==>
+    MEM prev (pred_labels (fn with fn_blocks := keep) lbl)
 Proof
   rpt strip_tac >>
-  simp[simplify_phi_inst_def] >>
-  qabbrev_tac `ops = phi_remove_non_preds preds inst.inst_operands` >>
-  `resolve_phi prev ops = SOME val_op` by (
-    fs[Abbr`ops`] >>
-    irule resolve_phi_remove_non_preds >> simp[]
-  ) >>
-  Cases_on `ops` >- fs[resolve_phi_def] >>
-  Cases_on `t` >- fs[resolve_phi_def] >>
-  Cases_on `t'`
-  >- (
-    fs[step_inst_def, Abbr`ops`] >>
-    Cases_on `h` >> fs[resolve_phi_def] >>
-    Cases_on `s' = prev` >> fs[resolve_phi_def] >>
-    simp[eval_operand_def]
-  ) >>
-  fs[step_inst_def]
-QED
-*)
-
-(* ===== Simplify-PHI preserves block labels ===== *)
-
-Theorem simplify_phi_block_label:
-  !preds bb. (simplify_phi_block preds bb).bb_label = bb.bb_label
-Proof
-  rw[simplify_phi_block_def]
+  fs[pred_labels_def, MEM_MAP, MEM_FILTER] >>
+  qexists_tac `bb` >>
+  simp[MEM_FILTER] >>
+  metis_tac[]
 QED
 
-(* ===== Simplify-PHI preserves step_in_block ===== *)
-
-Theorem step_in_block_simplify_phi:
-  !fn bb s preds res is_term.
-    step_in_block fn bb s = (res, is_term) /\
-    s.vs_prev_bb <> NONE /\
-    preds = pred_labels fn bb.bb_label /\
-    (!idx inst prev out val_op.
-       get_instruction bb idx = SOME inst /\
-       inst.inst_opcode = PHI /\
-       inst.inst_outputs = [out] /\
-       s.vs_prev_bb = SOME prev /\
-       MEM prev preds /\
-       resolve_phi prev inst.inst_operands = SOME val_op ==>
-       result_equiv_cfg (step_inst (simplify_phi_inst preds inst) s)
-                        (step_inst inst s))
-  ==>
-    ?res'. step_in_block fn (simplify_phi_block preds bb) s = (res', is_term) /\
-           result_equiv_cfg res' res
-Proof
-  cheat
-QED
-
-(* TODO: proof attempt
+Theorem block_last_inst_terminator:
+  !bb idx inst.
+    block_terminator_last bb /\
+    get_instruction bb idx = SOME inst /\
+    is_terminator inst.inst_opcode ==>
+    block_last_inst bb = SOME inst
 Proof
   rpt strip_tac >>
-  fs[step_in_block_def, simplify_phi_block_def] >>
-  Cases_on `get_instruction bb s.vs_inst_idx` >> fs[] >>
-  rename1 `get_instruction bb _ = SOME inst` >>
-  `get_instruction (bb with bb_instructions := MAP (simplify_phi_inst preds) bb.bb_instructions) s.vs_inst_idx =
-   SOME (simplify_phi_inst preds inst)` by (
-    rw[get_instruction_def] >> simp[EL_MAP]
-  ) >>
-  simp[] >>
-  Cases_on `step_inst inst s` >> fs[] >>
-  simp[step_inst_def] >>
-  (* Non-PHI instructions are unchanged *)
-  Cases_on `inst.inst_opcode = PHI` >> fs[] >>
-  first_x_assum (qspecl_then [`s.vs_inst_idx`, `inst`] mp_tac) >> simp[] >>
-  strip_tac >> simp[]
-QED
-*)
-
-(* ===== run_block equivalence for simplify_phi_block ===== *)
-
-Theorem run_block_simplify_phi:
-  !fn bb s preds.
-    s.vs_prev_bb <> NONE /\
-    preds = pred_labels fn bb.bb_label /\
-    (!idx inst prev out val_op.
-       get_instruction bb idx = SOME inst /\
-       inst.inst_opcode = PHI /\
-       inst.inst_outputs = [out] /\
-       s.vs_prev_bb = SOME prev /\
-       MEM prev preds /\
-       resolve_phi prev inst.inst_operands = SOME val_op ==>
-       result_equiv_cfg (step_inst (simplify_phi_inst preds inst) s)
-                        (step_inst inst s))
-  ==>
-    result_equiv_cfg (run_block fn (simplify_phi_block preds bb) s)
-                     (run_block fn bb s)
-Proof
-  cheat
+  fs[block_terminator_last_def] >>
+  qpat_x_assum `get_instruction _ _ = _` mp_tac >>
+  simp[get_instruction_def] >> strip_tac >>
+  `bb.bb_instructions <> []` by (Cases_on `bb.bb_instructions` >> fs[]) >>
+  simp[block_last_inst_def, listTheory.LAST_EL, arithmeticTheory.PRE_SUB1] >>
+  simp[] >> metis_tac[]
 QED
 
-(* TODO: proof attempt
+Theorem run_block_ok_successor:
+  !fn bb s s'.
+    cfg_wf fn /\
+    MEM bb fn.fn_blocks /\
+    run_block fn bb s = OK s' /\
+    ~s'.vs_halted ==>
+    MEM s'.vs_current_bb (block_successors bb)
 Proof
-  ho_match_mp_tac run_block_ind >>
-  rpt gen_tac >> strip_tac >>
-  rpt gen_tac >> strip_tac >>
+  ho_match_mp_tac run_block_ind >> rpt strip_tac >>
   qpat_x_assum `run_block _ _ _ = _` mp_tac >>
   simp[Once run_block_def] >>
   Cases_on `step_in_block fn bb s` >> Cases_on `q` >> simp[] >>
-  strip_tac >>
-  drule step_in_block_simplify_phi >>
-  disch_then (qspecl_then [`preds`] mp_tac) >> simp[] >>
-  disch_then (fn th => simp[th]) >>
-  simp[Once run_block_def]
+  Cases_on `v.vs_halted` >> simp[] >>
+  Cases_on `r` >> simp[] >- (
+    (* Terminator case *)
+    qpat_x_assum `step_in_block _ _ _ = _` mp_tac >>
+    simp[step_in_block_def] >>
+    Cases_on `get_instruction bb s.vs_inst_idx` >> simp[] >>
+    Cases_on `step_inst x s` >> simp[] >>
+    Cases_on `is_terminator x.inst_opcode` >> simp[] >>
+    strip_tac >>
+    `block_terminator_last bb` by
+      (fs[cfg_wf_def] >> metis_tac[]) >>
+    drule_at (Pos last) block_last_inst_terminator >> simp[] >>
+    simp[block_successors_def] >>
+    drule_at (Pos last) step_inst_terminator_successor >> simp[]
+  ) >>
+  (* Non-terminal case *)
+  first_x_assum irule >> simp[]
 QED
-*)
+
+Theorem reachable_label_step:
+  !fn entry src dst.
+    reachable_label fn entry src /\ cfg_edge fn src dst ==>
+    reachable_label fn entry dst
+Proof
+  rw[reachable_label_def] >>
+  irule relationTheory.RTC_TRANS >>
+  qexists_tac `src` >>
+  conj_tac >- simp[] >>
+  irule (CONJUNCT2 (SPEC (cfg_edge fn) relationTheory.RTC_RULES)) >>
+  simp[]
+QED
+
+Theorem run_function_remove_unreachable_equiv:
+  !fuel fn s.
+    cfg_wf fn /\
+    phi_fn_wf fn /\
+    reachable_label fn (entry_label fn) s.vs_current_bb /\
+    (s.vs_prev_bb = NONE ==> s.vs_current_bb = entry_label fn) /\
+    (s.vs_prev_bb = SOME prev ==> MEM prev (pred_labels fn s.vs_current_bb)) /\
+    (s.vs_prev_bb = SOME prev ==> reachable_label fn (entry_label fn) prev)
+  ==>
+    result_equiv_cfg (run_function fuel fn s)
+                     (run_function fuel (remove_unreachable_blocks fn) s)
+Proof
+  Induct_on `fuel` >> rpt strip_tac
+  >- simp[run_function_def, result_equiv_cfg_def] >>
+  simp[Once run_function_def] >>
+  Cases_on `lookup_block s.vs_current_bb fn.fn_blocks`
+  >- (
+    qabbrev_tac `entry = entry_label fn` >>
+    qabbrev_tac `keep = FILTER (\\bb. reachable_label fn entry bb.bb_label) fn.fn_blocks` >>
+    qabbrev_tac `fn_keep = fn with fn_blocks := keep` >>
+    qabbrev_tac `fix = MAP (\\bb. simplify_phi_block (pred_labels fn_keep bb.bb_label) bb) keep` >>
+    `remove_unreachable_blocks fn = fn with fn_blocks := fix` by
+      (simp[remove_unreachable_blocks_def, Abbr`entry`, Abbr`keep`,
+            Abbr`fn_keep`, Abbr`fix`, LET_THM, cfg_wf_def]) >>
+    simp[Once run_function_def] >>
+    `lookup_block s.vs_current_bb keep = NONE` by
+      (irule lookup_block_filter_none >> simp[Abbr`keep`]) >>
+    `lookup_block s.vs_current_bb fix = NONE` by
+      (drule lookup_block_simplify_phi_block_none >> simp[Abbr`fix`]) >>
+    simp[result_equiv_cfg_def]
+  )
+  >- (
+    rename1 `lookup_block _ _ = SOME bb` >>
+    qabbrev_tac `entry = entry_label fn` >>
+    qabbrev_tac `keep = FILTER (\\bb. reachable_label fn entry bb.bb_label) fn.fn_blocks` >>
+    qabbrev_tac `fn_keep = fn with fn_blocks := keep` >>
+    qabbrev_tac `fix = MAP (\\bb. simplify_phi_block (pred_labels fn_keep bb.bb_label) bb) keep` >>
+    `remove_unreachable_blocks fn = fn with fn_blocks := fix` by
+      (simp[remove_unreachable_blocks_def, Abbr`entry`, Abbr`keep`,
+            Abbr`fn_keep`, Abbr`fix`, LET_THM, cfg_wf_def]) >>
+    `lookup_block s.vs_current_bb keep = SOME bb` by (
+      irule lookup_block_filter >> simp[Abbr`keep`] >>
+      `bb.bb_label = s.vs_current_bb` by metis_tac[lookup_block_label] >>
+      simp[]
+    ) >>
+    `lookup_block s.vs_current_bb fix =
+       SOME (simplify_phi_block (pred_labels fn_keep s.vs_current_bb) bb)` by
+      (simp[Abbr`fix`] >> drule lookup_block_simplify_phi_block >> simp[]) >>
+    simp[Once run_function_def] >>
+    Cases_on `s.vs_prev_bb`
+    >- (
+      `s.vs_current_bb = entry` by metis_tac[] >>
+      `bb = HD fn.fn_blocks` by
+        (irule lookup_block_at_hd >> simp[Abbr`entry`, cfg_wf_def]) >>
+      `block_has_no_phi bb` by
+        (simp[Abbr`entry`] >> metis_tac[phi_fn_wf_entry_no_phi]) >>
+      `simplify_phi_block (pred_labels fn_keep bb.bb_label) bb = bb` by
+        simp[simplify_phi_block_no_phi] >>
+      simp[] >>
+      Cases_on `run_block fn bb s` >> simp[result_equiv_cfg_def] >>
+      rename1 `run_block fn bb s = OK v` >>
+      Cases_on `v.vs_halted` >> simp[result_equiv_cfg_def] >>
+      `v.vs_prev_bb = SOME s.vs_current_bb` by
+        (drule_all run_block_ok_prev_bb >> simp[]) >>
+      `MEM s.vs_current_bb (pred_labels fn v.vs_current_bb)` by (
+        `MEM bb fn.fn_blocks` by metis_tac[lookup_block_MEM] >>
+        drule_all run_block_ok_successor >> strip_tac >>
+        drule pred_labels_mem_from_edge >> simp[]
+      ) >>
+      `reachable_label fn entry v.vs_current_bb` by (
+        `MEM bb fn.fn_blocks` by metis_tac[lookup_block_MEM] >>
+        drule_all run_block_ok_successor >> strip_tac >>
+        `cfg_edge fn s.vs_current_bb v.vs_current_bb` by
+          (rw[cfg_edge_def] >> qexists_tac `bb` >> simp[]) >>
+        metis_tac[reachable_label_step]
+      ) >>
+      first_x_assum irule >>
+      simp[Abbr`entry`] >>
+      metis_tac[]
+    )
+    >- (
+      rename1 `s.vs_prev_bb = SOME prev` >>
+      `result_equiv_cfg (run_block fn bb s)
+         (run_block fn (simplify_phi_block (pred_labels fn_keep bb.bb_label) bb) s)` by (
+        `phi_block_wf (pred_labels fn bb.bb_label) bb` by
+          (irule phi_fn_wf_block >> simp[]) >>
+        `MEM prev (pred_labels fn_keep bb.bb_label)` by
+          (irule pred_labels_keep_reachable >> simp[Abbr`keep`]) >>
+        `!lbl. MEM lbl (pred_labels fn_keep bb.bb_label) ==>
+              MEM lbl (pred_labels fn bb.bb_label)` by
+          (rpt strip_tac >>
+           irule pred_labels_subset >>
+           simp[Abbr`fn_keep`] >>
+           metis_tac[]) >>
+        irule run_block_simplify_phi >>
+        simp[] >> metis_tac[]
+      ) >>
+      Cases_on `run_block fn bb s` >>
+      Cases_on `run_block fn (simplify_phi_block (pred_labels fn_keep bb.bb_label) bb) s` >>
+      gvs[result_equiv_cfg_def] >>
+      rename1 `run_block fn bb s = OK v` >>
+      `v.vs_halted <=> v'.vs_halted` by fs[state_equiv_cfg_def] >>
+      Cases_on `v.vs_halted` >> gvs[result_equiv_cfg_def] >>
+      `run_block fn (simplify_phi_block (pred_labels fn_keep bb.bb_label) bb) s = OK v` by (
+        irule run_block_simplify_phi_ok >>
+        `phi_block_wf (pred_labels fn bb.bb_label) bb` by
+          (irule phi_fn_wf_block >> simp[]) >>
+        `MEM prev (pred_labels fn_keep bb.bb_label)` by
+          (irule pred_labels_keep_reachable >> simp[Abbr`keep`]) >>
+        `!lbl. MEM lbl (pred_labels fn_keep bb.bb_label) ==>
+              MEM lbl (pred_labels fn bb.bb_label)` by
+          (rpt strip_tac >>
+           irule pred_labels_subset >>
+           simp[Abbr`fn_keep`] >>
+           metis_tac[]) >>
+        simp[]
+      ) >>
+      `v.vs_prev_bb = SOME s.vs_current_bb` by
+        (drule_all run_block_ok_prev_bb >> simp[]) >>
+      `MEM s.vs_current_bb (pred_labels fn v.vs_current_bb)` by (
+        `MEM bb fn.fn_blocks` by metis_tac[lookup_block_MEM] >>
+        drule_all run_block_ok_successor >> strip_tac >>
+        drule pred_labels_mem_from_edge >> simp[]
+      ) >>
+      `reachable_label fn entry v.vs_current_bb` by (
+        `MEM bb fn.fn_blocks` by metis_tac[lookup_block_MEM] >>
+        drule_all run_block_ok_successor >> strip_tac >>
+        `cfg_edge fn s.vs_current_bb v.vs_current_bb` by
+          (rw[cfg_edge_def] >> qexists_tac `bb` >> simp[]) >>
+        metis_tac[reachable_label_step]
+      ) >>
+      first_x_assum irule >>
+      simp[Abbr`entry`] >>
+      metis_tac[]
+    )
+  )
+QED
 
 (* ===== Simplify-CFG Step Correctness (Skeletons) ===== *)
 
 Theorem remove_unreachable_blocks_correct:
-  !fn s fuel.
-    fn.fn_blocks <> [] /\
+  !fn s.
+    cfg_wf fn /\
+    phi_fn_wf fn /\
     s.vs_current_bb = entry_label fn /\
     s.vs_prev_bb = NONE ==>
-    result_equiv_cfg (run_function fuel fn s)
-                     (run_function fuel (remove_unreachable_blocks fn) s)
+    run_function_equiv_cfg fn (remove_unreachable_blocks fn) s
 Proof
-  cheat
-QED
-
-Theorem merge_blocks_correct:
-  !fn a_lbl b_lbl s fuel.
-    merge_blocks_cond fn a_lbl b_lbl /\
-    s.vs_current_bb = entry_label fn /\
-    s.vs_prev_bb = NONE ==>
-    result_equiv_cfg (run_function fuel fn s)
-                     (run_function fuel (merge_blocks fn a_lbl b_lbl) s)
-Proof
-  cheat
-QED
-
-Theorem merge_jump_correct:
-  !fn a_lbl b_lbl s fuel.
-    merge_jump_cond fn a_lbl b_lbl /\
-    s.vs_current_bb = entry_label fn /\
-    s.vs_prev_bb = NONE ==>
-    result_equiv_cfg (run_function fuel fn s)
-                     (run_function fuel (merge_jump fn a_lbl b_lbl) s)
-Proof
-  cheat
+  rw[run_function_equiv_cfg_def]
+  >- (
+    qexists_tac `fuel` >>
+    `result_equiv_cfg (run_function fuel fn s)
+                      (run_function fuel (remove_unreachable_blocks fn) s)` by (
+      irule run_function_remove_unreachable_equiv >>
+      simp[reachable_label_def, relationTheory.RTC_REFL]
+    ) >>
+    Cases_on `run_function fuel fn s` >>
+    gvs[terminates_def, result_equiv_cfg_def]
+  )
+  >- (
+    qexists_tac `fuel'` >>
+    `result_equiv_cfg (run_function fuel' fn s)
+                      (run_function fuel' (remove_unreachable_blocks fn) s)` by (
+      irule run_function_remove_unreachable_equiv >>
+      simp[reachable_label_def, relationTheory.RTC_REFL]
+    ) >>
+    Cases_on `run_function fuel' (remove_unreachable_blocks fn) s` >>
+    gvs[terminates_def, result_equiv_cfg_def]
+  )
 QED
 
 Theorem simplify_cfg_step_correct:
-  !fn fn' s fuel.
+  !fn fn' s.
     simplify_cfg_step fn fn' /\
-    fn.fn_blocks <> [] /\
+    cfg_wf fn /\
+    phi_fn_wf fn /\
     s.vs_current_bb = entry_label fn /\
-    s.vs_prev_bb = NONE ==>
-    result_equiv_cfg (run_function fuel fn s)
-                     (run_function fuel fn' s)
+    s.vs_prev_bb = NONE /\
+    s.vs_inst_idx = 0 ==>
+    run_function_equiv_cfg fn fn' s
 Proof
   cheat
 QED
 
 Theorem simplify_cfg_correct:
-  !fn fn' s fuel.
+  !fn fn' s.
     simplify_cfg fn fn' /\
-    fn.fn_blocks <> [] /\
+    cfg_wf fn /\
+    phi_fn_wf fn /\
     s.vs_current_bb = entry_label fn /\
-    s.vs_prev_bb = NONE ==>
-    result_equiv_cfg (run_function fuel fn s)
-                     (run_function fuel fn' s)
+    s.vs_prev_bb = NONE /\
+    s.vs_inst_idx = 0 ==>
+    run_function_equiv_cfg fn fn' s
 Proof
   cheat
 QED
